\begin{equation}
    E = \frac{1}{2} \sum_{i}{(y_i - \overline{y_i})^2} =
    \frac{1}{2} \left[ (y_1 - \overline{y_1})^2 + (y_2 - \overline{y_2})^2 \right]
\end{equation}

\begin{equation*}
    \frac{\partial E}{\partial y_1} = \overline{y_1} - y_1
    \qquad % horizontal space
    \frac{\partial E}{\partial y_2} = \overline{y_2} - y_2
\end{equation*}

\begin{equation}
    \overline{y_1} = \frac{1}{1+ e^{-o_1}}
    \qquad % horizontal space
    \overline{y_2} = \frac{1}{1+ e^{-o_2}}
\end{equation}

\begin{equation*}
    \frac{\partial \overline{y_1}}{\partial o_1} = \overline{y_1} (1 - \overline{y_1})
    \qquad % horizontal space
    \frac{\partial \overline{y_2}}{\partial o_2} = \overline{y_2} (1 - \overline{y_2})
\end{equation*}

\begin{equation*}
    \frac{\partial E}{\partial o_1} =
    \frac{\partial E}{\partial \overline{y_1}} \frac{\partial \overline{y_1}}{\partial o_1}
    \qquad % horizontal space
    \frac{\partial E}{\partial o_2} =
    \frac{\partial E}{\partial \overline{y_2}} \frac{\partial \overline{y_2}}{\partial o_2}
\end{equation*}

\begin{equation}
    o_1 =  z_1 w_{11}^2 + z_2 w_{21}^2 + b_2 w_{31}^2
    \qquad % horizontal space
    o_2 =  z_1 w_{12}^2 + z_2 w_{22}^2 + b_2 w_{32}^2
\end{equation}

\begin{equation*}
    \frac{\partial o_1}{\partial w_{11}^2} = z_1
    \qquad % horizontal space
    \frac{\partial o_1}{\partial w_{21}^2} = z_2
    \qquad % horizontal space
    \frac{\partial o_1}{\partial z_1} = w_{11}^2
    \qquad % horizontal space
    \frac{\partial o_1}{\partial z_2} = w_{21}^2
\end{equation*}

\begin{equation*}
    \frac{\partial o_2}{\partial w_{12}^2} = z_1
    \qquad % horizontal space
    \frac{\partial o_2}{\partial w_{22}^2} = z_2
    \qquad % horizontal space
    \frac{\partial o_2}{\partial z_1} = w_{12}^2
    \qquad % horizontal space
    \frac{\partial o_2}{\partial z_2} = w_{22}^2
\end{equation*}

\begin{equation*}
    \frac{\partial E}{\partial z_1} =
    \frac{\partial E}{\partial o_1} \frac{\partial o_1}{\partial z_1} +
    \frac{\partial E}{\partial o_2} \frac{\partial o_2}{\partial z_1}
\end{equation*}

\begin{equation*}
    \frac{\partial E}{\partial z_2} =
    \frac{\partial E}{\partial o_1} \frac{\partial o_1}{\partial z_2} +
    \frac{\partial E}{\partial o_2} \frac{\partial o_2}{\partial z_2}
\end{equation*}

\begin{equation}
    z_1 = \frac{1}{1+ e^{-h_1}}
    \qquad % horizontal space
    z_2 = \frac{1}{1+ e^{-h_2}}
\end{equation}

\begin{equation*}
    \frac{\partial z_1}{\partial h_1} = z_1 (1 - z_1)
    \qquad % horizontal space
    \frac{\partial z_2}{\partial h_2} = z_2 (1 - z_2)
\end{equation*}

\begin{equation}
    h_1 =  x_1 w_{11}^1 + x_2 w_{21}^1 + b_1 w_{31}^1
    \qquad % horizontal space
    h_2 =  x_1 w_{12}^1 + x_2 w_{22}^1 + b_1 w_{32}^1
\end{equation}

\begin{equation*}
    \frac{\partial h_1}{\partial w_{11}^1} = x_1
    \qquad % horizontal space
    \frac{\partial h_1}{\partial w_{21}^1} = x_2
\end{equation*}

\begin{equation*}
    \frac{\partial h_2}{\partial w_{12}^1} = x_1
    \qquad % horizontal space
    \frac{\partial h_2}{\partial w_{22}^1} = x_2
\end{equation*}
